src/proofs/no_slashable_attestations/supporting_lemmas/fnc_invs_1_26.dfy
@@ -2087,52 +2087,52 @@ module Fnc_Invs_1_26
         assert process' == ret_check_for_next_queued_duty.state;        
     }  
 
-    lemma lemma_inv22_add_block_to_bn(
+    lemma lemma_inv_no_active_consensus_instance_before_receiving_att_duty_add_block_to_bn(
         s: DVCState,
         block: BeaconBlock,
         s': DVCState 
     )
     requires add_block_to_bn.requires(s, block)
     requires s' == add_block_to_bn(s, block)    
-    requires inv22_body(s)
-    ensures inv22_body(s')
+    requires inv_no_active_consensus_instance_before_receiving_att_duty_body(s)
+    ensures inv_no_active_consensus_instance_before_receiving_att_duty_body(s')
     { }
 
-    lemma lemma_inv22_f_listen_for_attestation_shares(
+    lemma lemma_inv_no_active_consensus_instance_before_receiving_att_duty_f_listen_for_attestation_shares(
         process: DVCState,
         attestation_share: AttestationShare,
         process': DVCState
     )
     requires f_listen_for_attestation_shares.requires(process, attestation_share)
     requires process' == f_listen_for_attestation_shares(process, attestation_share).state        
-    requires inv22_body(process)
-    ensures inv22_body(process')
+    requires inv_no_active_consensus_instance_before_receiving_att_duty_body(process)
+    ensures inv_no_active_consensus_instance_before_receiving_att_duty_body(process')
     {}
 
-    lemma lemma_inv22_f_start_next_duty(process: DVCState, attestation_duty: AttestationDuty, process': DVCState)
+    lemma lemma_inv_no_active_consensus_instance_before_receiving_att_duty_f_start_next_duty(process: DVCState, attestation_duty: AttestationDuty, process': DVCState)
     requires f_start_next_duty.requires(process, attestation_duty)
     requires process' == f_start_next_duty(process, attestation_duty).state   
-    requires inv22_body(process)
-    ensures inv22_body(process')
+    requires inv_no_active_consensus_instance_before_receiving_att_duty_body(process)
+    ensures inv_no_active_consensus_instance_before_receiving_att_duty_body(process')
     { } 
 
-    lemma lemma_inv22_f_resend_attestation_share(
+    lemma lemma_inv_no_active_consensus_instance_before_receiving_att_duty_f_resend_attestation_share(
         process: DVCState,
         process': DVCState)
     requires f_resend_attestation_share.requires(process)
     requires process' == f_resend_attestation_share(process).state        
-    requires inv22_body(process)
-    ensures inv22_body(process')
+    requires inv_no_active_consensus_instance_before_receiving_att_duty_body(process)
+    ensures inv_no_active_consensus_instance_before_receiving_att_duty_body(process')
     { } 
 
-    lemma lemma_inv22_f_check_for_next_queued_duty(
+    lemma lemma_inv_no_active_consensus_instance_before_receiving_att_duty_f_check_for_next_queued_duty(
         process: DVCState,
         process': DVCState
     )
     requires f_check_for_next_queued_duty.requires(process)
     requires process' == f_check_for_next_queued_duty(process).state    
-    requires inv22_body(process)
-    ensures inv22_body(process')
+    requires inv_no_active_consensus_instance_before_receiving_att_duty_body(process)
+    ensures inv_no_active_consensus_instance_before_receiving_att_duty_body(process')
     decreases process.attestation_duties_queue
     {
         if  && process.attestation_duties_queue != [] 
@@ -2154,16 +2154,16 @@ module Fnc_Invs_1_26
                             new_attestation_slashing_db
                         )                        
                     );
-                    lemma_inv22_f_check_for_next_queued_duty(process_mod, process');
+                    lemma_inv_no_active_consensus_instance_before_receiving_att_duty_f_check_for_next_queued_duty(process_mod, process');
                 }
                 else
                 { 
                     var process_mod := process.(
                         attestation_duties_queue := process.attestation_duties_queue[1..]
                     );     
-                    assert inv22_body(process_mod);
+                    assert inv_no_active_consensus_instance_before_receiving_att_duty_body(process_mod);
 
-                    lemma_inv22_f_start_next_duty(process_mod, process.attestation_duties_queue[0], process');
+                    lemma_inv_no_active_consensus_instance_before_receiving_att_duty_f_start_next_duty(process_mod, process.attestation_duties_queue[0], process');
                 }
         }
         else
@@ -2172,7 +2172,7 @@ module Fnc_Invs_1_26
         }
     }
 
-    lemma lemma_inv22_f_att_consensus_decided(
+    lemma lemma_inv_no_active_consensus_instance_before_receiving_att_duty_f_att_consensus_decided(
         process: DVCState,
         id: Slot,
         decided_attestation_data: AttestationData, 
@@ -2180,8 +2180,8 @@ module Fnc_Invs_1_26
     )
     requires f_att_consensus_decided.requires(process, id, decided_attestation_data)
     requires process' == f_att_consensus_decided(process, id, decided_attestation_data).state         
-    requires inv22_body(process)
-    ensures inv22_body(process')
+    requires inv_no_active_consensus_instance_before_receiving_att_duty_body(process)
+    ensures inv_no_active_consensus_instance_before_receiving_att_duty_body(process')
     {
         
         if  || !process.current_attestation_duty.isPresent()
@@ -2215,24 +2215,24 @@ module Fnc_Invs_1_26
             );
 
     
-        assert inv22_body(process);
+        assert inv_no_active_consensus_instance_before_receiving_att_duty_body(process);
 
         var ret_check_for_next_queued_duty := f_check_for_next_queued_duty(process);
         
-        lemma_inv22_f_check_for_next_queued_duty(process, ret_check_for_next_queued_duty.state);
+        lemma_inv_no_active_consensus_instance_before_receiving_att_duty_f_check_for_next_queued_duty(process, ret_check_for_next_queued_duty.state);
 
         assert process' == ret_check_for_next_queued_duty.state;        
     } 
     
-    lemma lemma_inv22_f_listen_for_new_imported_blocks(
+    lemma lemma_inv_no_active_consensus_instance_before_receiving_att_duty_f_listen_for_new_imported_blocks(
         process: DVCState,
         block: BeaconBlock,
         process': DVCState
     )
     requires f_listen_for_new_imported_blocks.requires(process, block)
     requires process' == f_listen_for_new_imported_blocks(process, block).state        
-    requires inv22_body(process)
-    ensures inv22_body(process')
+    requires inv_no_active_consensus_instance_before_receiving_att_duty_body(process)
+    ensures inv_no_active_consensus_instance_before_receiving_att_duty_body(process')
     {
         var new_consensus_instances_already_decided := f_listen_for_new_imported_blocks_helper_1(process, block);
 
@@ -2252,7 +2252,7 @@ module Fnc_Invs_1_26
                     rcvd_attestation_shares := process.rcvd_attestation_shares - att_consensus_instances_already_decided.Keys                    
                 );    
         
-        assert inv22_body(process);
+        assert inv_no_active_consensus_instance_before_receiving_att_duty_body(process);
 
         if process.current_attestation_duty.isPresent() && process.current_attestation_duty.safe_get().slot in att_consensus_instances_already_decided
         {
@@ -2267,32 +2267,32 @@ module Fnc_Invs_1_26
                 )                
             );
             
-            assert inv22_body(process);
+            assert inv_no_active_consensus_instance_before_receiving_att_duty_body(process);
 
-            lemma_inv22_f_check_for_next_queued_duty(process, process');
+            lemma_inv_no_active_consensus_instance_before_receiving_att_duty_f_check_for_next_queued_duty(process, process');
         }
         else
         {               
-            assert inv22_body(process);
+            assert inv_no_active_consensus_instance_before_receiving_att_duty_body(process);
         }
     } 
 
-    lemma lemma_inv22_f_serve_attestation_duty(
+    lemma lemma_inv_no_active_consensus_instance_before_receiving_att_duty_f_serve_attestation_duty(
         process: DVCState,
         attestation_duty: AttestationDuty,
         process': DVCState
     )  
     requires f_serve_attestation_duty.requires(process, attestation_duty)
     requires process' == f_serve_attestation_duty(process, attestation_duty).state
-    requires inv22_body(process)
-    ensures inv22_body(process')
+    requires inv_no_active_consensus_instance_before_receiving_att_duty_body(process)
+    ensures inv_no_active_consensus_instance_before_receiving_att_duty_body(process')
     {
         var process_mod := process.(
                 attestation_duties_queue := process.attestation_duties_queue + [attestation_duty],
                 all_rcvd_duties := process.all_rcvd_duties + {attestation_duty}
             );        
         
-        lemma_inv22_f_check_for_next_queued_duty(process_mod, process');        
+        lemma_inv_no_active_consensus_instance_before_receiving_att_duty_f_check_for_next_queued_duty(process_mod, process');        
     } 
 
     lemma lemma_inv_slot_of_active_consensus_instance_is_lower_than_slot_of_latest_served_att_duty_add_block_to_bn(
@@ -2334,7 +2334,7 @@ module Fnc_Invs_1_26
     requires process' == f_check_for_next_queued_duty(process).state        
     requires inv17_body(process)
     requires inv18_body(process)
-    requires inv22_body(process)
+    requires inv_no_active_consensus_instance_before_receiving_att_duty_body(process)
     requires inv_slot_of_active_consensus_instance_is_lower_than_slot_of_latest_served_att_duty_body(process)
     ensures inv_slot_of_active_consensus_instance_is_lower_than_slot_of_latest_served_att_duty_body(process')
     decreases process.attestation_duties_queue
@@ -2447,7 +2447,7 @@ module Fnc_Invs_1_26
     requires inv14_body(process, attestation_duty)
     requires inv17_body(process)
     requires inv18_body(process)
-    requires inv22_body(process)    
+    requires inv_no_active_consensus_instance_before_receiving_att_duty_body(process)    
     requires inv_slot_of_active_consensus_instance_is_lower_than_slot_of_latest_served_att_duty_body(process)
     ensures inv_slot_of_active_consensus_instance_is_lower_than_slot_of_latest_served_att_duty_body(process')
     {
@@ -2460,7 +2460,7 @@ module Fnc_Invs_1_26
         assert inv7_body(process_mod);
         assert inv17_body(process_mod);                        
         assert inv18_body(process_mod);         
-        assert inv22_body(process_mod);         
+        assert inv_no_active_consensus_instance_before_receiving_att_duty_body(process_mod);         
         assert inv_slot_of_active_consensus_instance_is_lower_than_slot_of_latest_served_att_duty_body(process_mod);
         
         lemma_inv_slot_of_active_consensus_instance_is_lower_than_slot_of_latest_served_att_duty_f_check_for_next_queued_duty(process_mod, process');        
@@ -2475,7 +2475,7 @@ module Fnc_Invs_1_26
     requires process' == f_listen_for_new_imported_blocks(process, block).state        
     requires inv17_body(process)
     requires inv18_body(process)
-    requires inv22_body(process)
+    requires inv_no_active_consensus_instance_before_receiving_att_duty_body(process)
     requires inv_slot_of_active_consensus_instance_is_lower_than_slot_of_latest_served_att_duty_body(process)
     ensures inv_slot_of_active_consensus_instance_is_lower_than_slot_of_latest_served_att_duty_body(process')
     {
@@ -2499,7 +2499,7 @@ module Fnc_Invs_1_26
         
         assert inv17_body(process_mod);
         assert inv18_body(process_mod);
-        assert inv22_body(process_mod);
+        assert inv_no_active_consensus_instance_before_receiving_att_duty_body(process_mod);
         assert inv_slot_of_active_consensus_instance_is_lower_than_slot_of_latest_served_att_duty_body(process_mod);
 
         if process_mod.current_attestation_duty.isPresent() && process_mod.current_attestation_duty.safe_get().slot in att_consensus_instances_already_decided
@@ -2517,7 +2517,7 @@ module Fnc_Invs_1_26
             
             assert inv17_body(temp_process);
             assert inv18_body(temp_process);
-            assert inv22_body(temp_process);
+            assert inv_no_active_consensus_instance_before_receiving_att_duty_body(temp_process);
             assert inv_slot_of_active_consensus_instance_is_lower_than_slot_of_latest_served_att_duty_body(temp_process);
 
             lemma_inv_slot_of_active_consensus_instance_is_lower_than_slot_of_latest_served_att_duty_f_check_for_next_queued_duty(temp_process, process');
@@ -2540,7 +2540,7 @@ module Fnc_Invs_1_26
     requires process' == f_att_consensus_decided(process, id, decided_attestation_data).state         
     requires inv17_body(process)
     requires inv18_body(process)
-    requires inv22_body(process)
+    requires inv_no_active_consensus_instance_before_receiving_att_duty_body(process)
     requires inv_slot_of_active_consensus_instance_is_lower_than_slot_of_latest_served_att_duty_body(process)
     ensures inv_slot_of_active_consensus_instance_is_lower_than_slot_of_latest_served_att_duty_body(process')
     {
@@ -2577,7 +2577,7 @@ module Fnc_Invs_1_26
 
         assert inv17_body(process_mod);
         assert inv18_body(process_mod);
-        assert inv22_body(process_mod);
+        assert inv_no_active_consensus_instance_before_receiving_att_duty_body(process_mod);
         assert inv_slot_of_active_consensus_instance_is_lower_than_slot_of_latest_served_att_duty_body(process_mod);
 
         var ret_check_for_next_queued_duty := f_check_for_next_queued_duty(process_mod);
