src/proofs/no_slashable_attestations/supporting_lemmas/proofs_ind_inv.dfy
@@ -82,7 +82,7 @@ module Proofs_DV_Ind_Inv
     {        
         &&  inv19(dv)           
         &&  inv21(dv) 
-        &&  inv22(dv)      
+        &&  inv_no_active_consensus_instance_before_receiving_att_duty(dv)      
         &&  inv_slot_of_active_consensus_instance_is_lower_than_slot_of_latest_served_att_duty(dv)  
         &&  inv_consensus_instance_only_for_slot_in_which_dvc_has_rcvd_att_duty(dv)          
         &&  inv_consensus_instances_only_for_rcvd_duties(dv)  
@@ -193,12 +193,12 @@ module Proofs_DV_Ind_Inv
     ensures inv19(dv')        
     ensures inv20(dv, dv')
     ensures inv21(dv')
-    ensures inv22(dv')
+    ensures inv_no_active_consensus_instance_before_receiving_att_duty(dv')
     {
         lemma_inv19_dv_next(dv, e, dv');
         lemma_inv20_dv_next(dv, e, dv');
         lemma_inv21_dv_next(dv, e, dv');        
-        lemma_inv22_dv_next(dv, e, dv');                
+        lemma_inv_no_active_consensus_instance_before_receiving_att_duty_dv_next(dv, e, dv');                
         // lemma_inv_slot_of_active_consensus_instance_is_lower_than_slot_of_latest_served_att_duty_dv_next(dv, e, dv');                
         // lemma_inv_consensus_instance_only_for_slot_in_which_dvc_has_rcvd_att_duty_dv_next(dv, e, dv');    
         // lemma_inv_consensus_instances_only_for_rcvd_duties_dv_next(dv, e, dv');    
